LambdaGraph.lean
@@ -1,6 +1,9 @@
 -- This module serves as the root of the `LambdaGraph` library.
 -- Import modules here that should be built as part of the library.
-import LambdaGraph.Basic
-import LambdaGraph.Nest
-import LambdaGraph.Subst
-import LambdaGraph.Step
+
+module
+
+public import LambdaGraph.Basic
+public import LambdaGraph.Nest
+public import LambdaGraph.Subst
+public import LambdaGraph.Step
